.

theories/Data/Vector.v
@@ -7,6 +7,43 @@ Require Import DschingisKhan.Prelude.PreludeUtil.
 
 Module MyFin.
 
+  Definition evalFin {n : nat} (i : Fin n) : nat := proj1_sig (runFin i).
+
+  Lemma evalFin_unfold {n : nat} (i : Fin n) :
+    evalFin i =
+    match i with
+    | FZ => O
+    | FS i' => S (evalFin i')
+    end.
+  Proof. destruct i; reflexivity. Qed.
+
+  Lemma evalFin_inj {n : nat} (i1 : Fin n) (i2 : Fin n)
+    (hyp_eq : evalFin i1 = evalFin i2)
+    : i1 = i2.
+  Proof.
+    unfold evalFin in hyp_eq.
+    rewrite <- getFin_runFin_id with (i := i1).
+    rewrite <- getFin_runFin_id with (i := i2).
+    destruct (runFin i1) as [m1 hyp_lt1].
+    destruct (runFin i2) as [m2 hyp_lt2].
+    cbn in *. subst m1. eapply eq_congruence, le_pirrel.
+  Qed.
+
+  Definition incrFin {m : nat} : forall n : nat, Fin m -> Fin (n + m) :=
+    fix incrFin_fix (n : nat) (i : Fin m) {struct n} : Fin (n + m) :=
+    match n as x return Fin (x + m) with
+    | O => i
+    | S n' => FS (incrFin_fix n' i)
+    end
+  .
+
+  Lemma incrFin_spec {m : nat} (n : nat) (i : Fin m)
+    : evalFin (incrFin n i) = n + evalFin i.
+  Proof with eauto.
+    induction n as [ | n IH]; simpl...
+    rewrite evalFin_unfold. eapply eq_congruence...
+  Qed.
+
 End MyFin.
 
 Module MyVec.
